module sets where

data _and_ : Set → Set → Set where
    and-def : {x y : Set} → x → y → x and y
infixl 40 _and_

data _≡_ : Set → Set → Set where
    ≡-def : {x y : Set} → (x → y) and (y → x) → x ≡ y
infixr 30 _≡_

straight : {x y : Set} → x ≡ y → x → y
straight (≡-def (and-def z _)) = z

back : {x y : Set} → x ≡ y → y → x
back (≡-def (and-def _ z)) = z

data ∃ : {x : Set} → (z : x → Set) → Set where
    ∃-def : {x : Set} → (y : x) → (z : x → Set) → z y → ∃ z
    
postulate
    𝕊 : Set
    _∈_ : 𝕊 → 𝕊 → Set
infix 50 _∈_

data _==_ : 𝕊 → 𝕊 → Set where
    ==-def : (x y z : 𝕊) → (z ∈ x ≡ z ∈ y) → x == y
infixr 50 _==_

postulate
    eq_ax : (x y : 𝕊) → (x == y) → (z : 𝕊) → (x ∈ z ≡ y ∈ z)
    pair_ax : (x y : 𝕊) → ∃ λ { z → x ∈ z and y ∈ z }
    ∪ : 𝕊 → 𝕊 -- union axiom
    ∪-def : (x y : 𝕊) → (∃ λ { z → x ∈ z and z ∈ y }) ≡ x ∈ ∪ y

data _⊆_ : 𝕊 → 𝕊 → Set where
    ⊆-def : (x y : 𝕊) → ((z : 𝕊) → z ∈ x → z ∈ y) → x ⊆ y 
infixr 50 _⊆_

postulate
    𝓟 : 𝕊 → 𝕊 -- power axiom
    𝓟-def : (x y : 𝕊) → x ⊆ y ≡ x ∈ (𝓟 y)

data ⊥ : Set where

data ¬ : Set → Set where
    ¬-def : (x : Set) → (x → ⊥) → ¬ x 
    
th-1 : (x y : 𝕊) → x ⊆ y → (∪ x) ⊆ (∪ y)
th-1 x y (⊆-def _ _ z) = ⊆-def (∪ x) (∪ y) λ w i → straight (∪-def w y) (lm-1 w (back (∪-def w x) i))
    where lm-1 : (a : 𝕊) → ∃ (λ { α → a ∈ α and α ∈ x }) → ∃ (λ { α → a ∈ α and α ∈ y })
          lm-1 a (∃-def b _ (and-def c d)) = ∃-def b (λ α → a ∈ α and α ∈ y) (and-def c (z b d))

th-2 : (x : 𝕊) → x ⊆ 𝓟 (∪ x)
th-2 x = ⊆-def x (𝓟 (∪ x)) λ y z → straight (𝓟-def y (∪ x)) (⊆-def y (∪ x) λ w i → straight (∪-def w x) (∃-def y (λ j → w ∈ j and j ∈ x) (and-def i z)))

th-3 : (x : 𝕊) → ∪ x ⊆ x → ∪ (𝓟 x) ⊆ 𝓟 x
th-3 x (⊆-def .(∪ x) .x y) =
    ⊆-def (∪ (𝓟 x)) (𝓟 x) λ z w → straight (𝓟-def z x) (⊆-def z x (λ i j → y i (straight (∪-def i x) (∃-def z (λ { α → i ∈ α and α ∈ x }) (and-def j (lm-2 z (back (∪-def z (𝓟 x)) w)))))))
    where lm-1 : (a b : 𝕊) → a ⊆ b → (α : 𝕊) → α ∈ a → α ∈ b
          lm-1 _ _ (⊆-def c _ d) α β = d α β
          lm-2 : (z : 𝕊) → ∃ (λ { α → z ∈ α and α ∈ 𝓟 x }) → z ∈ x 
          lm-2 z (∃-def a _ (and-def b c)) = lm-1 a x ((back (𝓟-def a x)) c) z b
